proofs/isabelle/SpecRest/core/Translate.thy
@@ -52,5 +52,7 @@ fun translate :: "expr \<Rightarrow> smt_term" where
 | "translate (StrLit v _)                  = TStrLit v"
 | "translate (SeqEmpty _)                  = TSeqEmpty"
 | "translate (SeqCons e rest _)            = TSeqCons (translate e) (translate rest)"
+| "translate (MapEmpty _)                  = TMapEmpty"
+| "translate (MapCons k v rest _)          = TMapCons (translate k) (translate v) (translate rest)"
 
 end
