proofs/isabelle/SpecRest/core/IR_Lower.thy
@@ -31,6 +31,8 @@ and lower_with_assigns ::
        \<Rightarrow> expr \<Rightarrow> option_span \<Rightarrow> expr option"
 and lowerSeqList ::
     "String.literal list \<Rightarrow> expr_full list \<Rightarrow> option_span \<Rightarrow> expr option"
+and lowerMapEntries ::
+    "String.literal list \<Rightarrow> map_entry_full list \<Rightarrow> option_span \<Rightarrow> expr option"
 where
   "lower _ (BoolLitF b sp)     = Some (BoolLit b sp)"
 | "lower _ (IntLitF n sp)      = Some (IntLit n sp)"
@@ -41,7 +43,6 @@ where
 | "lower _ (LambdaF _ _ _)     = None"
 | "lower _ (CallF _ _ _)       = None"
 | "lower _ (ConstructorF _ _ _)     = None"
-| "lower _ (MapLiteralF _ _)        = None"
 | "lower _ (SetComprehensionF _ _ _ _) = None"
 | "lower _ (TheF _ _ _ _)      = None"
 | "lower _ (MatchesF _ _ _)    = None"
@@ -183,6 +184,7 @@ where
       | Some base' \<Rightarrow> lower_with_assigns enums updates base' sp)"
 | "lower enums (SetLiteralF elems sp) = lowerSetList enums elems sp"
 | "lower enums (SeqLiteralF elems sp) = lowerSeqList enums elems sp"
+| "lower enums (MapLiteralF entries sp) = lowerMapEntries enums entries sp"
 | "lower enums (IfF c a b sp) =
      (case (lower enums c, lower enums a, lower enums b) of
         (Some c', Some a', Some b') \<Rightarrow> Some (Ite c' a' b' sp)
@@ -206,6 +208,12 @@ where
      (case (lower enums e, lowerSeqList enums rest sp) of
         (Some e', Some s') \<Rightarrow> Some (SeqCons e' s' sp)
       | _ \<Rightarrow> None)"
+
+| "lowerMapEntries _ [] sp = Some (MapEmpty sp)"
+| "lowerMapEntries enums (MapEntryFull k v _ # rest) sp =
+     (case (lower enums k, lower enums v, lowerMapEntries enums rest sp) of
+        (Some k', Some v', Some m') \<Rightarrow> Some (MapCons k' v' m' sp)
+      | _ \<Rightarrow> None)"
   by pat_completeness auto
 
 termination
@@ -214,12 +222,14 @@ termination
                Inl (Inl (_, e)) \<Rightarrow> size e
              | Inl (Inr (_, elems, _)) \<Rightarrow> size_list size elems
              | Inr (Inl (_, updates, _, _)) \<Rightarrow> size_list size updates
-             | Inr (Inr (_, elems, _)) \<Rightarrow> size_list size elems),
+             | Inr (Inr (Inl (_, elems, _))) \<Rightarrow> size_list size elems
+             | Inr (Inr (Inr (_, entries, _))) \<Rightarrow> size_list size entries),
         (\<lambda>p. case p of
                Inl (Inl _) \<Rightarrow> 0
              | Inl (Inr (_, elems, _)) \<Rightarrow> Suc (length elems)
              | Inr (Inl (_, updates, _, _)) \<Rightarrow> Suc (length updates)
-             | Inr (Inr (_, elems, _)) \<Rightarrow> Suc (length elems))
+             | Inr (Inr (Inl (_, elems, _))) \<Rightarrow> Suc (length elems)
+             | Inr (Inr (Inr (_, entries, _))) \<Rightarrow> Suc (length entries))
        ]")
      auto
 
